code/hash-new/Hacl.Hash.Common.fsti
@@ -9,7 +9,6 @@ module ST = FStar.HyperStack.ST
 module M = LowStar.Modifies
 module B = LowStar.Buffer
 module Spec = Spec.Hash.Common
-
 open Spec.Hash.Helpers
 
 (** We need to reveal the definition of the internal state for clients to use it *)
@@ -38,8 +37,10 @@ let size_len_ul (a: hash_alg): n:U32.t { U32.v n = size_len_8 a } =
   | MD5 | SHA1 | SHA2_224 | SHA2_256 -> 8ul
   | SHA2_384 | SHA2_512 -> 16ul
 
+(* Padding, not specialized, to be inlined in a specialized caller instead. *)
+
 inline_for_extraction
-let pad_t (a: hash_alg) = len:len_t a -> dst:B.buffer U8.t ->
+let pad_st (a: hash_alg) = len:len_t a -> dst:B.buffer U8.t ->
   ST.Stack unit
     (requires (fun h ->
       len_v a len < max_input8 a /\
@@ -49,10 +50,20 @@ let pad_t (a: hash_alg) = len:len_t a -> dst:B.buffer U8.t ->
       M.(modifies (loc_buffer dst) h0 h1) /\
       Seq.equal (B.as_seq h1 dst) (Spec.pad a (len_v a len))))
 
-let hash_t (a: hash_alg) = b:B.buffer U8.t { B.length b = size_hash a }
+noextract
+val pad: a:hash_alg -> pad_st a
+
+(* So that the caller can compute which length to allocate for padding. *)
+
+val pad_len: a:hash_alg -> len:len_t a ->
+  x:U32.t { U32.v x = pad_length a (len_v a len) }
+
+let hash_st (a: hash_alg) = b:B.buffer U8.t { B.length b = size_hash a }
+
+(* Finish, not specialized, to be inlined in a specialized caller instead. *)
 
 inline_for_extraction
-let finish_t (a: hash_alg) = s:state a -> dst:hash_t a -> ST.Stack unit
+let finish_st (a: hash_alg) = s:state a -> dst:hash_st a -> ST.Stack unit
   (requires (fun h ->
     B.disjoint s dst /\
     B.live h s /\
@@ -60,3 +71,6 @@ let finish_t (a: hash_alg) = s:state a -> dst:hash_t a -> ST.Stack unit
   (ensures (fun h0 _ h1 ->
     M.(modifies (loc_buffer dst) h0 h1) /\
     Seq.equal (B.as_seq h1 dst) (Spec.finish a (B.as_seq h0 s))))
+
+noextract
+val finish: a:hash_alg -> finish_st a
